WIP on automatic index selection improvements.

src/QueryStructure/Automation/IndexSelection.v
@@ -10,20 +10,20 @@ Require Import Coq.Sorting.Mergesort Coq.Structures.Orders
         Fiat.QueryStructure.Automation.Common.
 
 Module AttrCountOrder <: TotalLeBool.
-  Definition t := (prod (string * (string * string)) nat).
+                          Definition t := (prod (string * (string * string)) nat).
 
-  (* Largest element first *)
-  Definition leb (x y : t) :=
-    leb (snd y) (snd x).
+                          (* Largest element first *)
+                          Definition leb (x y : t) :=
+                            leb (snd y) (snd x).
 
-  Theorem leb_total : forall a1 a2 : t, leb a1 a2 = true \/ leb a2 a1 = true.
-  Proof.
-    unfold t; intros; intuition; unfold leb; simpl.
-    case_eq (Compare_dec.leb b b0); intuition.
-    case_eq (Compare_dec.leb b0 b); intuition.
-    apply leb_iff_conv in H; apply leb_iff_conv in H0.
-    omega.
-  Qed.
+                          Theorem leb_total : forall a1 a2 : t, leb a1 a2 = true \/ leb a2 a1 = true.
+                          Proof.
+                            unfold t; intros; intuition; unfold leb; simpl.
+                            case_eq (Compare_dec.leb b b0); intuition.
+                            case_eq (Compare_dec.leb b0 b); intuition.
+                            apply leb_iff_conv in H; apply leb_iff_conv in H0.
+                            omega.
+                          Qed.
 
 End AttrCountOrder.
 
@@ -37,24 +37,28 @@ Record KindName
   := { KindNameKind : string;
        KindNameName : string }.
 
+Definition OccurenceCountT {n}
+           (qsSchema : Vector.t RawHeading n) :=
+  ilist (B := fun heading => list (prod string (Attributes heading))) qsSchema.
+
 Definition IncrementAttrCount
            (idx : string * (string * string))
            (cnt : RelationAttributeCounter.t nat)
-: RelationAttributeCounter.t nat :=
+  : RelationAttributeCounter.t nat :=
   match RelationAttributeCounter.find idx cnt with
-    | Some n => RelationAttributeCounter.add idx (S n) cnt
-    | _ => RelationAttributeCounter.add idx 1 cnt
+  | Some n => RelationAttributeCounter.add idx (S n) cnt
+  | _ => RelationAttributeCounter.add idx 1 cnt
   end.
 
 Definition CountAttributes (l : list (string * (string * string)))
-: list ((string * (string * string)) * nat)  :=
+  : list ((string * (string * string)) * nat)  :=
   sort (RelationAttributeCounter.elements
           (fold_right IncrementAttrCount
                       (RelationAttributeCounter.empty nat)
                       l)).
 
 (*Definition GetIndexes
-           (qs_schema : RawQueryStructureSchema)
+           (qsSchema : RawQueryStructureSchema)
            (indices : list ((string * (string * string)) * nat))
 : list (list (string * string)) :=
   map (fun ns : NamedSchema =>
@@ -63,122 +67,177 @@ Definition CountAttributes (l : list (string * (string * string)))
                                    then true
                                    else false)
                      indices))
-      (qschemaSchemas qs_schema). *)
+      (qschemaSchemas qsSchema). *)
 
-  Ltac TermAttributes Term :=
-    match Term with
-      | fun tups => @GetAttribute _ (@?f tups) ?BAidx =>
-        let Aidx := eval simpl in (bindex BAidx) in
-            match type of f with
-              | _ -> @Tuple (GetHeading _ ?Ridx) =>
-                constr:([(Ridx, Aidx)])
-            end
-    end.
+(* Add a new occurence to AttrCount *)
+Fixpoint InsertOccurence {n}
+         {qsSchema : Vector.t RawHeading n}
+         (idx : Fin.t n)
+         (NewOccurence : prod string (Attributes (Vector.nth qsSchema idx)))
+         (AttrCount : OccurenceCountT qsSchema)
+         {struct idx}
+  : OccurenceCountT qsSchema.
+Proof.
+  refine (match idx in (Fin.t m') return
+                forall (qsSchema : Vector.t _ m'),
+                  OccurenceCountT qsSchema
+                  -> prod string (Attributes (Vector.nth qsSchema idx))
+                  -> OccurenceCountT qsSchema with
+          | Fin.F1 q =>
+            fun v il new => _
+          | Fin.FS q p' =>
+            fun v il new => _
+          end qsSchema AttrCount NewOccurence).
+  - revert il new; pattern q, v; apply Vector.caseS; intros.
+    exact (icons (new :: ilist_hd il) (ilist_tl il)).
+  - revert p' il new; pattern q, v; apply Vector.caseS; intros.
+    exact (icons (ilist_hd il) (InsertOccurence _ _ p' new (ilist_tl il))).
+Defined.
 
-  Ltac ClauseAttributes WhereClause kTerm k :=
+Arguments InsertOccurence [_ _ _] _ _.
+Fixpoint MergeOccurence {n}
+         (qsSchema : Vector.t RawHeading n)
+         (AttrCount1 AttrCount2 : OccurenceCountT qsSchema)
+         {struct qsSchema}
+  : OccurenceCountT qsSchema :=
+  match qsSchema return
+        forall (AttrCount1 AttrCount2 : OccurenceCountT qsSchema),
+          OccurenceCountT qsSchema with
+  | Vector.nil => fun AttrCount1 AttrCount2 => inil
+  | Vector.cons _ _ qsSchema' =>
+    fun AttrCount1 AttrCount2 =>
+      icons (ilist_hd AttrCount1 ++ ilist_hd AttrCount2)
+            (MergeOccurence qsSchema' (ilist_tl AttrCount1) (ilist_tl AttrCount2))
+  end AttrCount1 AttrCount2.
+
+Arguments MergeOccurence [_ _] _ _.
+
+Fixpoint InitOccurence {n}
+         (qsSchema : Vector.t RawHeading n)
+         {struct qsSchema}
+  : OccurenceCountT qsSchema :=
+  match qsSchema return OccurenceCountT qsSchema with
+  | Vector.nil => inil
+  | Vector.cons _ _ qsSchema' =>
+    icons nil (InitOccurence qsSchema')
+  end.
+
+Definition GetOccurence {n}
+           {qsSchema : Vector.t RawHeading n}
+           (AttrCount : OccurenceCountT qsSchema)
+           (idx : Fin.t n)
+  : list (prod string (Attributes (Vector.nth qsSchema idx))) :=
+  ith AttrCount idx.
+
+Ltac TermAttributes Term k :=
+  match Term with
+  | fun tups => @GetAttributeRaw _ (@?f tups) ?BAidx =>
+    let Aidx := eval simpl in BAidx in
+        match type of f with
+        | _ -> @RawTuple (Vector.nth _ ?Ridx) =>
+          k Ridx Aidx
+        end
+  end.
+
+Ltac ClauseAttributes qsSchema WhereClause OtherClauses k :=
   match WhereClause with
-    | fun tups => @?C1 tups /\ @?C2 tups =>
-      ClauseAttributes C1 kTerm
-                       ltac:(fun attrs1 =>
-                               ClauseAttributes C2 kTerm
-                                                ltac:(fun attrs2 =>
-                                                        k (app attrs2 attrs1)))
-    | fun tups => @?C1 tups = @?C2 tups =>
-      let attrs1 := TermAttributes C1 in
-      let attrs2 := TermAttributes C2 in
-      k (map (fun a12 => (EqualityIndex, (fst a12, snd a12)))
-             (app attrs1 attrs2))
-    | fun tups => @?C1 tups = _ =>
-      let attrs1 := TermAttributes C1 in
-      k (map (fun a12 => (EqualityIndex, (fst a12, snd a12)))
-             (attrs1))
-    | fun tups => _ = @?C1 tups =>
-      let attrs1 := TermAttributes C1 in
-      k (map (fun a12 => (EqualityIndex, (fst a12, snd a12)))
-             (attrs1))
-    | _ => kTerm WhereClause k
-    | _ => k (@nil (string * (string * string)))
+  | fun tups => @?C1 tups /\ @?C2 tups =>
+    ClauseAttributes qsSchema C1 OtherClauses
+                     ltac:(fun attrs1 =>
+                             ClauseAttributes qsSchema C2 OtherClauses
+                                              ltac:(fun attrs2 =>
+                                                      k (MergeOccurence attrs2 attrs1)))
+  | fun tups => @?C1 tups = @?C2 tups =>
+    TermAttributes C1 ltac:(fun Ridx1 attr1 =>
+                              TermAttributes C2 ltac:(fun Ridx2 attr2 =>
+                                                        k (@InsertOccurence _ qsSchema Ridx1 (EqualityIndex, attr1) (@InsertOccurence _ qsSchema Ridx2 (EqualityIndex, attr2) (InitOccurence qsSchema)))))
+  | fun tups => @?C1 tups = _ =>
+    TermAttributes C1 ltac:(fun Ridx attr =>
+                              k (@InsertOccurence _ qsSchema Ridx (EqualityIndex, attr) (InitOccurence _)))
+  | fun tups => _ = @?C1 tups =>
+    TermAttributes C1 ltac:(fun Ridx attr =>
+                              k (@InsertOccurence _ qsSchema Ridx (EqualityIndex, attr) (InitOccurence _)))
+  | _ => OtherClauses WhereClause k
+  | _ => k (InitOccurence qsSchema)
   end.
 
-Ltac QueryAttributes QueryBody kTerm k :=
+Ltac QueryAttributes qsSchema QueryBody OtherClauses k :=
   match QueryBody with
-    | @UnConstrQuery_In _ ?qsSchema _ ?Ridx ?QueryBody' => (* Initial "Naked" Case *)
-      let Ridx' := eval simpl in (bindex Ridx) in
-          let QueryBody'' := eval cbv beta in (fun tup : @Tuple (GetHeading qsSchema Ridx') => QueryBody' tup) in
-              QueryAttributes QueryBody'' kTerm k  (* Simply recurse under binder *)
+  | @UnConstrQuery_In _ _ _ ?Ridx ?QueryBody' => (* Initial "Naked" Case *)
+    let Ridx' := eval compute in Ridx in
+        let QueryBody'' := eval cbv beta in (fun tup : @RawTuple (Vector.nth qsSchema Ridx') => QueryBody' tup) in
+            QueryAttributes qsSchema QueryBody'' OtherClauses k  (* Simply recurse under binder *)
 
-    | fun tups : ?A =>
-        @UnConstrQuery_In _ ?qsSchema _ ?Ridx
-                          (@?f tups) => (* Already Under binder *)
-      let Ridx' := eval simpl in (bindex Ridx) in
-      let join := eval cbv beta in
-      (fun joinedtups : prod A (@Tuple (GetHeading qsSchema Ridx')) =>
-         f (fst joinedtups) (snd joinedtups)) in
-          QueryAttributes join kTerm k
-    | fun tups => Where (@?P tups) (@?QueryBody' tups) =>
-      ClauseAttributes P kTerm
-                       ltac:(fun attrs =>
-                               QueryAttributes QueryBody' kTerm ltac:(fun attrs' => k (app attrs attrs')))
-    | _ => k (@nil (string * (string * string)))
+  | fun tups : ?A =>
+      @UnConstrQuery_In _ _ _ ?Ridx
+                        (@?f tups) => (* Already Under binder *)
+    let Ridx' := eval compute in Ridx in
+        let join := eval cbv beta in
+        (fun joinedtups : prod A (@RawTuple (Vector.nth qsSchema Ridx')) =>
+           f (fst joinedtups) (snd joinedtups)) in
+            QueryAttributes qsSchema join OtherClauses k
+  | fun tups => Where (@?P tups) (@?QueryBody' tups) =>
+    ClauseAttributes qsSchema P OtherClauses
+                     ltac:(fun attrs =>
+                             QueryAttributes qsSchema QueryBody' OtherClauses ltac:(fun attrs' => k (MergeOccurence attrs attrs')))
+  | _ => k (InitOccurence qsSchema)
   end.
 
-Ltac MethodAttributes meth kTerm l :=
+Ltac MethodAttributes meth qsSchema OtherClauses l :=
   hone method meth;
   [ match goal with
-        |- context[For ?Q] =>
-        QueryAttributes
-                 Q kTerm ltac:(fun attrs => let attrs' := eval simpl in attrs in
-                                          unify l attrs')
-      | _ => unify l (@nil (string * (string * string)))
+      |- context[For ?Q] =>
+      QueryAttributes qsSchema Q OtherClauses
+                      ltac:(fun attrs =>
+                              let l' := eval simpl in attrs in
+                                  unify l l')
+    | _ => unify l (InitOccurence qsSchema )
     end; finish honing | ].
 
-Ltac MethodsAttributes' meths kTerm l :=
+Ltac MethodsAttributes' meths qsSchema OtherClauses l :=
   match meths with
-    | cons ?meth ?meths' =>
-      makeEvar (list (string * (string * string)))
-               ltac:(fun l1 =>
-                       makeEvar (list (string * (string * string)))
-                                ltac:(fun l2 =>
-                                        unify l (app l1 l2);
-                                      MethodAttributes meth kTerm l1;
-                                      MethodsAttributes' meths' kTerm l2))
-    | nil => unify l (@nil (string * (string * string)))
+  | Vector.cons _ ?meth _ ?meths' =>
+    makeEvar (OccurenceCountT qsSchema)
+             ltac:(fun l1 =>
+                     makeEvar (OccurenceCountT qsSchema)
+                              ltac:(fun l2 =>
+                                      unify l (MergeOccurence l1 l2);
+                                    MethodAttributes meth qsSchema  OtherClauses l1;
+                                    MethodsAttributes' meths' qsSchema  OtherClauses l2))
+  | Vector.nil _ => unify l (InitOccurence qsSchema)
   end.
 
-(*Ltac GenerateIndexesFor meths kTerm k :=
+Ltac GenerateIndexesFor meths OtherClauses k :=
   match goal with
-      |- Sharpened
-           (@BuildADT (UnConstrQueryStructure ?qs_schema) _ _ _ _) =>
-      makeEvar (list (string * (string * string)))
-               ltac:(fun l =>
-                       MethodsAttributes' meths kTerm l;
-                     let l' := eval compute in
-                     (GetIndexes qs_schema (CountAttributes l)) in
-                         k l')
+    |- Sharpened
+         (@BuildADT (UnConstrQueryStructure ?qsSchema) _ _ _ _ _ _) =>
+    let rels := eval simpl in (Vector.map rawSchemaHeading (qschemaSchemas qsSchema)) in
+        makeEvar (OccurenceCountT rels)
+                 ltac:(fun l => MethodsAttributes' meths rels OtherClauses l; let l' := eval simpl in l in k l')
   end.
 
-Ltac GenerateIndexesForAll kTerm k :=
+Ltac GenerateIndexesForAll OtherClauses k :=
   match goal with
-      |- Sharpened
-           (@BuildADT (UnConstrQueryStructure ?qs_schema) _ ?methSigs _ _) =>
-      let meths := eval compute in (map methID methSigs) in
-          GenerateIndexesFor meths kTerm k
-  end. *)
+    |- Sharpened
+         (@BuildADT (UnConstrQueryStructure ?qsSchema) _ _ _ ?methSigs _ _) =>
+    let meths := eval compute in (Vector.map methID methSigs) in
+        GenerateIndexesFor meths OtherClauses k
+  end.
 
 Tactic Notation "make" "simple" "indexes" "using" constr(attrlist) :=
   match goal with
-    | [ |- Sharpened (@BuildADT (UnConstrQueryStructure ?sch) _ _ _ _ _ _ )] =>
-      let sch' := eval simpl in (qschemaSchemas sch) in
-          makeIndex' sch' attrlist
-                     ltac:(fun l =>
-                             pose_string_hyps; pose_heading_hyps;
-                           let index := fresh "Index" in
-                           pose l as index;
-                           simpl in index;
-                           pose_string_hyps_in index; pose_heading_hyps_in index;
-                           pose_search_term_in index;
-                           pose_SearchUpdateTerms_in index;
-                           hone representation using (@DelegateToBag_AbsR sch index))
+  | [ |- Sharpened (@BuildADT (UnConstrQueryStructure ?sch) _ _ _ _ _ _ )] =>
+    let sch' := eval simpl in (qschemaSchemas sch) in
+        makeIndex' sch' attrlist
+                   ltac:(fun l =>
+                           pose_string_hyps; pose_heading_hyps;
+                         let index := fresh "Index" in
+                         pose l as index;
+                         simpl in index;
+                         pose_string_hyps_in index; pose_heading_hyps_in index;
+                         pose_search_term_in index;
+                         pose_SearchUpdateTerms_in index;
+                         hone representation using (@DelegateToBag_AbsR sch index))
   end.
 
 (*Tactic Notation "make" "indexes" "using" tactic(ClauseMatchers) :=
@@ -189,12 +248,12 @@ Tactic Notation "make" "simple" "indexes" "using" constr(attrlist) :=
 (* Recurse over [fds] to find an attribute matching s *)
 Ltac findMatchingTerm fds kind s k :=
   match fds with
-    | ({| KindIndexKind := ?IndexType;
-          KindIndexIndex := ?fd |}, ?X) =>
-      (* Check if this field name is equal to s; process [X] with [k] if so. *)
-      pose fds;
+  | ({| KindIndexKind := ?IndexType;
+        KindIndexIndex := ?fd |}, ?X) =>
+    (* Check if this field name is equal to s; process [X] with [k] if so. *)
+    pose fds;
       unify s fd;
       unify kind IndexType;
       k X
-    | (?fds1, ?fds2) => findMatchingTerm fds1 kind s k || findMatchingTerm fds2 kind s k
+  | (?fds1, ?fds2) => findMatchingTerm fds1 kind s k || findMatchingTerm fds2 kind s k
   end.
